revised transcript API

src/tls/HSL.Transcript.fsti
@@ -54,21 +54,18 @@ module G = FStar.Ghost
 module HSM = Parsers.Handshake
 module HSM12 = Parsers.Handshake12
 module HSM13 = Parsers.Handshake13
-
 module PV = Parsers.ProtocolVersion
 module LP = LowParse.Low.Base
 module IncHash = EverCrypt.Hash.Incremental
 module HashDef = Spec.Hash.Definitions
-
 module R = MITLS.Repr
 module R_HS = MITLS.Repr.Handshake
-
 module R_CH = MITLS.Repr.ClientHello
 module CH = Parsers.ClientHello
-
 module R_SH = MITLS.Repr.ServerHello
 module SH = Parsers.ServerHello
-
+module Psks = Parsers.OfferedPsks
+module PB = ParsersAux.Binders
 
 //TODO: move to a separate module
 let repr_hs12 (b:R.const_slice) =
@@ -85,67 +82,6 @@ type bytes = FStar.Seq.seq uint_8
 let hs_ch = ch:HSM.handshake{HSM.M_client_hello? ch}
 let hs_sh = sh:HSM.handshake{HSM.M_server_hello? sh}
 
-/// `hs_tch`: Handshake message holding a truncated client hello
-///
-/// Truncated client hellos are related to pre-shared keys.
-/// See below for more details
-
-//TODO: fill this out with Tahina's definition
-val empty_binders (bs:Parsers.OfferedPsks_binders.offeredPsks_binders) : prop
-
-let is_tch (ch:hs_ch) =
-    let open Parsers.OfferedPsks in
-    let open Parsers.ClientHelloExtension in
-    let open Parsers.ClientHello in
-    let ch = HSM.M_client_hello?._0 ch in
-    Cons? ch.extensions /\
-    CHE_pre_shared_key? (List.last ch.extensions) /\
-    (let offeredPsks = CHE_pre_shared_key?._0 (List.last ch.extensions) in
-     empty_binders offeredPsks.binders
-     )
-let hs_tch = ch:hs_ch{ is_tch ch }
-
-noeq
-type pre_client_offer = {
-  version : Parsers.ProtocolVersion.protocolVersion;
-  random : Parsers.Random.random;
-  session_id : Parsers.SessionID.sessionID;
-  cipher_suites : CH.clientHello_cipher_suites;
-  compression_method : CH.clientHello_compression_method;
-  extensions : list Parsers.ClientHelloExtension.clientHelloExtension;
-  psks: option (Parsers.OfferedPsks.offeredPsks_identities & uint_32)
-}
-
-let offer_of (ch:hs_ch) : pre_client_offer =
-  let ch = HSM.M_client_hello?._0 ch in
-  let extensions, psks =
-    if Cons? CH.(ch.extensions) &&
-      Parsers.ClientHelloExtension.CHE_pre_shared_key? (List.last ch.CH.extensions)
-    then
-      let open Parsers.OfferedPsks in
-      let init = List.init ch.CH.extensions in
-      let o = Parsers.ClientHelloExtension.CHE_pre_shared_key?._0 (List.last ch.CH.extensions) in
-      let len = (offeredPsks_binders_size32 o.binders) in
-      init,
-      Some (o.identities, len)
-    else ch.CH.extensions, None
-  in
-  { version = CH.(ch.version);
-    random = CH.(ch.random);
-    session_id = CH.(ch.session_id);
-    cipher_suites = CH.(ch.cipher_suites);
-    compression_method = CH.(ch.compression_method);
-    extensions = extensions;
-    psks = psks
-  }
-
-let client_offer = co:pre_client_offer{exists (ch:hs_ch). offer_of ch == co}
-
-let client_hello_of_client_offer (co:client_offer)
-  : GTot (ch:hs_ch{ offer_of ch == co })
-  = let (| ch, _ |) = FStar.IndefiniteDescription.indefinite_description hs_ch (fun ch -> offer_of ch == co) in
-    ch
-
 /// `is_hrr`: For now, we assume the existence of a pure function to
 /// decide if a server-hello message is a hello-retry-request (hrr)
 // assume
@@ -161,17 +97,73 @@ type retry =
   hs_ch
   & hello_retry_request
 
-// /// `client_hello_has_psk`: A client hello has a pre-shared key if
-// ///    that mode appears in one of its extensions
-// let client_hello_has_psk (ch:CH.clientHello) =
-//   exists (ext:_).
-//     List.memP ext Parsers.ClientHello.(ch.extensions) /\
-//     Parsers.ClientHelloExtension.CHE_pre_shared_key? ext /\
-//     True (* what else do we need? e.g., that it has as many binders as ids? *)
+////////////////////////////////////////////////////////////////////////////////
+// Truncated client hellos
+////////////////////////////////////////////////////////////////////////////////
+
+/// `hs_tch`: Handshake message holding a truncated client hello
+///
+/// Truncated client hellos are related to pre-shared keys.
+///
+/// See https://tlswg.org/tls13-spec/draft-ietf-tls-tls13.html#rfc.section.4.2.11
+///
+/// Broadly, the server selects a particular PSK binder to validate.
+///
+/// Validation involves checking the hash of the transcript up to the
+/// truncated client hello under a PSK binder key. Note, this may be
+/// more than just the truncated client hello, since the transcript
+/// may also include a hello-retry request.
+///
+/// At the client side, in order to prepare the client hello message,
+/// the client prepares a draft client hello with default binders of
+/// the appropriate length. It then repeatedly hashes the truncation
+/// of this draft client hello to compute the binder values, each time
+/// perhaps using a different hashing algorithm (as determined by the
+/// PSK identity).
+
+let clientHello_with_binders = ch:hs_ch {
+  PB.has_binders ch
+}
+
+let binders_len = len:uint_32{
+  35 <= UInt32.v len /\
+  UInt32.v len <= 65537
+}
+
+/// TODO: check with Tahina how to implement this function
+val tch_binders_len (ch:clientHello_with_binders)
+  : Tot (b:binders_len {
+           UInt32.v b =
+           Psks.offeredPsks_binders_bytesize (PB.get_binders ch)
+         })
+
+/// TODO: how to prove this lemma? We'll need it for injectivity
+val tch_binder_len_equiv (ch0 ch1:clientHello_with_binders)
+  : Lemma
+    (requires
+       PB.truncate_clientHello_bytes ch0 ==
+       PB.truncate_clientHello_bytes ch1)
+    (ensures
+       tch_binders_len ch0 == tch_binders_len ch1)
+
+let hs_tch = tch:clientHello_with_binders{
+  PB.get_binders tch == PB.build_canonical_binders (tch_binders_len tch)
+}
+
+/// TODO: Still need to check with Tahina about how to kill these
+/// assumes using PB
+let truncate (ch:clientHello_with_binders)
+  : GTot hs_tch
+  = let cb = PB.build_canonical_binders (tch_binders_len ch) in
+    let tch = PB.set_binders ch cb in
+    assume (tch_binders_len ch == tch_binders_len tch);
+    assert (PB.has_binders tch);
+    assert (PB.get_binders tch == cb);
+    tch
+
 
 /// `nego_version`: This is to be provided eventually by a refactoring
 /// of the Negotiation module.
-// assume
 val nego_version (ch:hs_ch)
                  (sh:hs_sh)
        : PV.protocolVersion
@@ -238,7 +230,7 @@ type transcript_t =
 
   | TruncatedHello:
       retried:option retry ->
-      offer:client_offer ->
+      tch:hs_tch ->
       transcript_t
 
   | Transcript12:
@@ -269,88 +261,156 @@ let transcript_size (t:transcript_t) =
 let extensible (t:transcript_t) = transcript_size t < max_transcript_size - 1
 let ext_transcript_t = t:transcript_t{extensible t}
 
-val transcript_hash (a:HashDef.hash_alg) (t:transcript_t)
-  : GTot (b: HashDef.lbytes (HashDef.hash_length a))
+(* A depiction of the state machine for transcript hashes
 
-// /// `transcript_bytes`: The input of the hash algorithm computed by
-// /// concatenated the message formatting of the messages
-// val transcript_bytes (t:transcript_t)
-//   : GTot (b: bytes {
-//        Seq.length b <= (max_transcript_size + 4) * max_message_size
-//     })
+
+   Start None ----ch--> Hello None ch ---------------.-------------.
+      |                     ^                        |             |
+      |                     |                       sh13         sh12
+      |                  complete_tch (server only)  |             |
+      |                     |                        v             v
+      .---------tch---> TCH None tch         Transcript13 None ... Transcript12 None ...
+      |                                        |          ^           |          ^
+      |                                        |          |           |          |
+      |                                        .---hsm13--.           .---hsm12--.
+     hrr
+      |                               Transcript13 (Some hrr)
+      |                                |         ^    ^
+      |                                |         |    |
+      |                                .--hsm13--.   sh13
+      v                                               |
+   Start (Some hrr) --ch-> Hello (Some hrr) ch -------.
+      |                         ^
+      |                         |
+      |                       complete_tch
+      |                         |
+      .---------tch------> TCH (Some hrr) tch
+
+   The machine is roughly structured as two copies of the same
+   machine, related by a hello-retry-request (hrr) transition. Note,
+   hrr is only in TLS1.3---so once that transition is taken, one can
+   no longer reach that Transcript12 state.
+
+   One subtlety is that, in practice, the client side of the protocol
+   takes a slightly different path through the machine than the
+   server. In the upper half of the machine (i.e., before hrr), the
+   client does not know which hashing algorithm will be
+   negotiated. But, it still needs to construct offered psk binders
+   using truncated client hellos. So, an expected usage is that the
+   client creates many instances of the of the transcript hash for
+   each hash algorithm prescribed by each chosen binder; computes the
+   hash of the truncated client hello and then discards the
+   transcript. Later, if/when the server picks a particular hashing
+   algorithm/binder, the client constructs a new transcript instance
+   with that algorithm and moves from `Start None` to `Hello None ch`
+   atomically, rather than via the `TCH` state.
+
+   OTOH, once an hrr message is sent, the hashing algorithm is already
+   chosen by the server and the client can move to the `Hello` state
+   via `TCH` (in the bottom half of the picture), just as the server.
+
+ *)
+
+/// The state machine above is split into several transition functions
+/// for convenience and ease of typability (note, the labels that
+/// guard the transitions do not all have the same type)
 
 (** TRANSITIONS **)
 
-/// `extend_with_hsm`: The main transition function
-///
-///    Dictates which next state to transition to (if any) from a
-///    given transcript and a message
-let transition_hsm
-      (t:transcript_t)
-      (m:HSM.handshake)
-  : GTot (option transcript_t)
-  = match t, m with
-    | Start retry, HSM.M_client_hello ch ->
-      //Missing: consistency between retry and ch
-      Some (Hello retry m)
+noeq
+type retry_repr = {
+  b1:R.const_slice;
+  ch:(ch:R_HS.repr b1{R_HS.is_ch ch});
+  b2:R.const_slice;
+  hrr:(sh:R_HS.repr b2{R_HS.is_sh sh /\ is_hrr (R.value sh)})
+}
 
-    | Hello retry ch, HSM.M_server_hello sh ->
-      if None? retry
-      && is_hrr m
+let hs_ch_repr b = ch:R_HS.repr b { R_HS.is_ch ch }
+let hs_sh_repr b = sh:R_HS.repr b { R_HS.is_sh sh }
+
+noeq
+type label =
+  | HSM:
+       #b:R.const_slice ->
+       ch_sh:R_HS.repr b ->
+       label
+
+  | HRR:
+      #b1:R.const_slice ->
+      ch:hs_ch_repr b1 ->
+      #b2:R.const_slice ->
+      hrr:hs_sh_repr b2{is_hrr (R.value hrr)} ->
+      label
+
+  | TCH:
+      #b:R.const_slice ->
+      ch:hs_ch_repr b{PB.has_binders (R.value ch)} ->
+      label
+
+  | CompleteTCH:
+      #b:R.const_slice ->
+      ch:hs_ch_repr b{PB.has_binders (R.value ch)} ->
+      label
+
+  | HSM12:
+      #b:R.const_slice ->
+      hs12:repr_hs12 b ->
+      label
+
+  | HSM13:
+      #b:R.const_slice ->
+      hs13:repr_hs13 b ->
+      label
+
+let transition (t:ext_transcript_t) (l:label)
+  : GTot (option transcript_t)
+  = match t, l with
+    | Start None, HRR ch sh ->
+      Some (Start (Some (R.value ch, R.value sh)))
+
+    | Start retry, HSM ch_sh ->
+      if R_HS.is_ch ch_sh
+      then Some (Hello retry (R.value ch_sh))
+      else None
+
+    | Start retry, TCH tch ->
+      Some (TruncatedHello retry (truncate (R.value tch)))
+
+    | TruncatedHello retry tch, CompleteTCH ch ->
+      if tch = truncate (R.value ch)
+      then Some (Hello retry (R.value ch))
+      else None
+
+    | Hello retry ch, HSM ch_sh ->
+      if not (R_HS.is_sh ch_sh)
       then None
       else
-        begin
-        match nego_version ch m, retry with
-        | PV.TLS_1p2, None ->
-          Some (Transcript12 ch m [])
+        let sh = R.value ch_sh in
+        if None? retry
+        && is_hrr sh
+        then None
+        else
+          begin
+          match nego_version ch sh, retry with
+          | PV.TLS_1p2, None ->
+            Some (Transcript12 ch sh [])
 
-        | PV.TLS_1p3, _ ->
-          Some (Transcript13 retry ch m [])
+          | PV.TLS_1p3, _ ->
+            Some (Transcript13 retry ch sh [])
 
-        | _ -> None
-        end
+          | _ -> None
+          end
 
-    | _ ->
-      None
+    | Transcript12 ch sh rest, HSM12 m ->
+      List.append_length rest [R.value m];
+      Some (Transcript12 ch sh (List.snoc (rest, R.value m)))
 
-/// `transition_hrr`:
-///    An auxiliary transition function, specific to TLS1.3
-///    that handles hello-retry requests
-let transition_hrr
-       (t:transcript_t)
-       (ch:HSM.handshake)
-       (sh:HSM.handshake) =
-  match t, ch, sh with
-  | Start None, HSM.M_client_hello _, HSM.M_server_hello _ ->
-    if is_hrr sh
-    then Some (Start (Some (ch, sh)))
-    else None
-  | _ ->
-    None
-
-/// `transition_hsm12`:
-///    An auxiliary transition function, specific to TLS1.2
-///    It only enforces the length constraint on the suffix
-let transition_hsm12 (t:ext_transcript_t) (m:HSM12.handshake12)
-  : option transcript_t
-  = match t with
-    | Transcript12 ch sh rest ->
-      List.append_length rest [m];
-      Some (Transcript12 ch sh (List.snoc (rest, m)))
+    | Transcript13 retry ch sh rest, HSM13 m ->
+      List.append_length rest [R.value m];
+      Some (Transcript13 retry ch sh (List.snoc (rest, R.value m)))
 
     | _ -> None
 
-/// `transition_hsm13`:
-///    An auxiliary transition function, specific to TLS1.3
-///    It only enforces the length constraint on the suffix
-let transition_hsm13 (t:ext_transcript_t) (m:HSM13.handshake13)
-  : option transcript_t
-  = match t with
-    | Transcript13 retry ch sh rest ->
-      List.append_length rest [m];
-      Some (Transcript13 retry ch sh (List.snoc (rest, m)))
-
-    | _ -> None
 
 (*** Concrete state and transitions ***)
 
@@ -421,154 +481,75 @@ val create (r:Mem.rgn) (a:HashDef.hash_alg)
          B.fresh_loc (footprint s) h0 h1)
 
 (** CONCRETE STATE TRANSITIONS **)
-/// `extend_pre_common`: Every state transition
-/// has some basic requirements
-///   -- state machine invariant
-///   -- validity of message representations
-///   -- disjointness of machine state and representation state
-///   -- extensibility of the transcript
-unfold
-let extend_pre_common
-  #a (s:state a)
-  #t (#b:R.const_slice) (r:R.repr t b)
-  (tx:transcript_t) (h:HS.mem)
-  = invariant s tx h /\
-    R.valid r h /\
-    B.loc_disjoint (C.loc_buffer R.(b.base)) (footprint s) /\
-    extensible tx
 
-/// `extend_hash_post_common`: Every state transition
-/// has some basic guarantees
-///   -- state machine invariant
-///   -- mutates only the state machine's footprint
-unfold
-let extend_post_common
-  #a (s:state a) (t:transcript_t) (h0 h1:HS.mem)
-  = invariant s t h1 /\
-    B.modifies (footprint s) h0 h1
+/// `valid_label`: Validity of the labels is simply the validity of
+///  the message representations it contains
+let valid_label (l:label) (h:HS.mem) =
+  match l with
+  | HSM ch_sh -> R.valid ch_sh h
+  | HRR ch hrr -> R.valid ch h /\ R.valid hrr h
+  | TCH ch -> R.valid ch h
+  | CompleteTCH ch -> R.valid ch h
+  | HSM12 hs12 -> R.valid hs12 h
+  | HSM13 hs13 -> R.valid hs13 h
 
-/// `extend_hsm`: The main transition
-///    - the state evolves according to `transition_hsm`
-val extend_hsm
-  (#a:_) (s:state a)
-  (#b:R.const_slice) (r:R_HS.repr b)
-  (tx:G.erased transcript_t)
+/// `loc_of_label`: The footprint of a label is simply the union of
+///  the footprints of all the message representations it contains
+let loc_of_label (l:label) =
+  match l with
+  | HRR #b1 _ #b2 _ ->
+    B.loc_union
+      (C.loc_buffer R.(b1.base))
+      (C.loc_buffer R.(b1.base))
+
+  | HSM #b _
+  | TCH #b _
+  | CompleteTCH #b _
+  | HSM12 #b _
+  | HSM13 #b _ ->
+    C.loc_buffer R.(b.base)
+
+/// `extend`: The single, concrete state transition function
+///
+///   `extend s l tx` transitions and returns the new state tx'
+///    in case the transition is enabled.
+///
+///    Internally, it extends the running hash of the transcript
+///
+///    It requires
+///      -- state machine invariant
+///      -- validity of message representations in the label
+///      -- disjointness of machine state and label state
+///      -- extensibility of the transcript
+///      -- and that the transition be enabled
+///
+///    It ensures
+///      -- state machine invariant
+///      -- that it mutates only the state machine's footprint
+///      -- that the new state is the one computed by the transition
+val extend (#a:_) (s:state a) (l:label) (tx:G.erased transcript_t)
   : Stack (G.erased transcript_t)
     (requires fun h ->
-      let tx = G.reveal tx in
-      extend_pre_common s r tx h /\
-      Some? (transition_hsm tx (R.value r)))
+        let tx = G.reveal tx in
+        invariant s tx h /\
+        valid_label l h /\
+        B.loc_disjoint (loc_of_label l) (footprint s) /\
+        extensible tx /\
+        Some? (transition tx l))
     (ensures fun h0 tx' h1 ->
-      let tx = G.reveal tx in
-      let tx' = G.reveal tx' in
-      tx' == Some?.v (transition_hsm tx (R.value r)) /\
-      extend_post_common s tx' h0 h1)
+        let tx = G.reveal tx in
+        let tx' = G.reveal tx' in
+        invariant s tx' h1 /\
+        B.modifies (footprint s) h0 h1 /\
+        tx' == Some?.v (transition tx l))
 
-/// `extend_hsm12`: Append to Transcript12
-///    - the state evolves according to `transition_hsm12`
-val extend_hsm12
-  (#a:_) (s:state a)
-  (#b:R.const_slice) (r:repr_hs12 b)
-  (tx:G.erased transcript_t)
-  : Stack (G.erased transcript_t)
-    (requires fun h ->
-      let tx = G.reveal tx in
-      extend_pre_common s r tx h /\
-      Some? (transition_hsm12 tx (R.value r)))
-    (ensures fun h0 tx' h1 ->
-      let tx = G.reveal tx in
-      let tx' = G.reveal tx' in
-      tx' == Some?.v (transition_hsm12 tx (R.value r)) /\
-      extend_post_common s tx' h0 h1)
 
-/// `extend_hsm13`: Append to Transcript13
-///    - the state evolves according to `transition_hsm13`
-val extend_hsm13
-  (#a:_) (s:state a)
-  (#b:R.const_slice) (r:repr_hs13 b)
-  (tx:G.erased transcript_t)
-  : Stack (G.erased transcript_t)
-    (requires fun h ->
-      let tx = G.reveal tx in
-      extend_pre_common s r tx h /\
-      Some? (transition_hsm13 tx (R.value r)))
-    (ensures fun h0 tx' h1 ->
-      let tx = G.reveal tx in
-      let tx' = G.reveal tx' in
-      tx' == Some?.v (transition_hsm13 tx (R.value r)) /\
-      extend_post_common s tx' h0 h1)
+(*** Hashes and injectivity ***)
 
-/// `extend_ch_with_psk`:
-///
-///    This is a specialized transition used by the server to process
-///    client hello's with pre-shared key binders.
-///
-///    See https://tlswg.org/tls13-spec/draft-ietf-tls-tls13.html#rfc.section.4.2.11
-///
-///    Broadly, the server selects a particular PSK binder to validate.
-///
-///    Validation involves checking the hash of the transcript up to
-///    the truncated client hello under a PSK binder key. Note, this
-///    may be more than just the truncated client hello, since the
-///    transcript may als include a hello-retry request.
-///
-///    This function does the following:
-///
-///      - truncates the client hello (until just before the first PSK
-///        binder)
-///
-///      - extends the transcript hash with the truncation, extracts
-///        that hash to a freshly allocation on the stack (in the
-///        caller's stack frame; note the `StackInline`)
-///
-///      - then extends the transcript hash to with the suffix of the
-///        client hello (i.e., all the binders excluded by the truncation)
-///
-///      - and correspondingly transitions the state machine to
-///        include the entire client hello
-val extend_ch_with_psk
-  (#a:_) (s:state a)
-  (#b:R.slice) (r:R_HS.repr b)
-  (tx:G.erased transcript_t)
-  : StackInline
-      (Hacl.Hash.Definitions.hash_t a &
-       G.erased transcript_t)
-    (requires fun h ->
-      let tx = G.reveal tx in
-      let hs = R.value r in
-      extend_pre_common s r tx h /\
-      Start? tx /\
-      HSM.M_client_hello? hs /\
-      client_hello_has_psk (HSM.M_client_hello?._0 hs))
-    (ensures fun h0 (hash, tx') h1 ->
-      let tx = G.reveal tx in
-      let tx' = G.reveal tx' in
-      B.fresh_loc (B.loc_buffer hash) h0 h1 /\
-      B.live h1 hash /\
-      tx' == Hello (Start?.retried tx) (R.value r) /\
-      extend_post_common s tx' h0 h1)
+/// `transcript_hash`: The specificational hash of the transcript
+val transcript_hash (a:HashDef.hash_alg) (t:transcript_t)
+  : GTot (b: HashDef.lbytes (HashDef.hash_length a))
 
-/// `extend_hrr`: Hello retry requests
-///     See https://tlswg.org/tls13-spec/draft-ietf-tls-tls13.html#rfc.section.4.1.4
-///  Transitions according to `transition_hrr`
-val extend_hrr
-  (#a:_) (s:state a)
-  (#b:R.slice) (r_ch:R_HS.repr b)
-  (#b':R.slice) (r_sh:R_HS.repr b')
-  (tx:G.erased transcript_t)
-  : Stack (G.erased transcript_t)
-    (requires fun h ->
-      let tx = G.reveal tx in
-      extend_pre_common s r_ch tx h /\
-      extend_pre_common s r_sh tx h /\
-      Some? (transition_hrr tx (R.value r_ch) (R.value r_sh)))
-    (ensures fun h0 tx' h1 ->
-      let tx = G.reveal tx in
-      let tx' = G.reveal tx' in
-      tx' == Some?.v (transition_hrr tx (R.value r_ch) (R.value r_sh)) /\
-      extend_post_common s tx' h0 h1)
-
-(*** Extracting hashes and injectivity ***)
 
 /// `extract_hash`:
 ///
@@ -582,28 +563,36 @@ val extract_hash
   (tag:Hacl.Hash.Definitions.hash_t a)
   (tx:G.erased transcript_t)
   : Stack unit
-    (requires (fun h0 ->
+    (requires fun h0 ->
       let tx = G.reveal tx in
       invariant s tx h0 /\
       B.live h0 tag /\
-      B.loc_disjoint (footprint s) (B.loc_buffer tag)))
-    (ensures (fun h0 _ h1 ->
+      B.loc_disjoint (footprint s) (B.loc_buffer tag))
+    (ensures fun h0 _ h1 ->
       let open B in
       let tx = G.reveal tx in
       invariant s tx h1 /\
       modifies (loc_union (footprint s) (loc_buffer tag)) h0 h1 /\
       B.live h1 tag /\
-      B.as_seq h1 tag == Spec.Hash.hash a (transcript_bytes tx)))
+      B.as_seq h1 tag == transcript_hash a tx)
 
 
 /// `injectivity`: The main lemma provided by this module is a form of
 ///  collision resistance adapted to transcripts, i.e., if the hashes
 ///  of two transcripts match then the transcripts themselves do.
-val injectivity (a:HashDef.hash_alg) (tx1 tx2:G.erased transcript_t)
-  : Lemma
-    (ensures (
-      let tx1 = G.reveal tx1 in
-      let tx2 = G.reveal tx2 in
-      Spec.Hash.hash a (transcript_bytes tx1) ==
-      Spec.Hash.hash a (transcript_bytes tx2) ==>
-      tx1 == tx2))
+
+/// TODO, still need to understand how to state this in terms of
+/// Hashing.CRF
+///
+/// Something like
+
+// val injectivity (a:HashDef.hash_alg) (tx1 tx2:G.erased transcript_t)
+//   : Stack unit
+//     (requires fun h ->
+//       hashed a tx1 /\
+//       hashed a tx2)
+//     (ensures fun h0 _ h1 ->
+//       h0 == h1 /\
+//       (crf a /\
+//        transcript_hash a tx1 == transcript_hash a tx2 ==>
+//        tx1 == tx2))
